Further work on Fragmenta reppository

Haskell/FragmentaTests/FrPersonVehicleMotor/FrPersonVehicleMotor.hs
@@ -1,0 +1,72 @@
+--------------------------
+-- Project: PCs/Fragmenta
+-- Module: 'SGTest2'
+-- Description: Batch of tests exercising features of SGs and SG refinement
+-- Author: Nuno Amálio
+---------------------------
+import SGrs
+import Grs
+import CheckUtils
+import System.Environment
+import Control.Monad(when)
+import FrParsing
+import MyMaybe
+import LoadCheckDraw
+import Utils
+
+def_path = "FragmentaTests/FrPersonVehicleMotor/"
+img_path = "FragmentaTests/FrPersonVehicleMotor/img/"
+
+saveDrawings = do
+   draw_mdl def_path img_path "PersonVehicleAny"
+   draw_mdl def_path img_path "PersonVehicleMotor"
+   draw_def def_path img_path "Person_Vehicle_Motor.fr"
+
+check_PVA = do
+    amdl<-load_mdl_def def_path "PersonVehicleAny"
+    check_report_wf "PersonVehicleAny" (Just Total) amdl True
+
+check_PVM = do
+    mdl<-load_mdl_def def_path "PersonVehicleMotor"
+    check_report_wf "PersonVehicleMotor" (Just Total) mdl True
+
+-- Checks the well-formedness of the abstract model
+do_test1 = do
+   (nmaf, af)<-load_fr_def def_path "Person_Vehicle_AnyM.fr"
+   check_report_wf nmaf (Just Total) af True
+
+-- Checks the well-formedness of the concrete fragment against the abstract one
+do_test2 = do
+   (nmaf, af)<-load_fr_def def_path "Person_Vehicle_AnyM.fr"
+   (nmf, f)<-load_fr_def def_path "Person_Vehicle_Motor.fr"
+   (nm_m1, m1)<-load_morphism_def def_path "m_PVI.gm"
+   check_report_wf nmaf (Just Total) af True
+   check_report_wf nmf (Just Total) f True
+   check_morphism (nm_m1++ " refinement morphism (Weak)") (Just WeakM) f m1 af True
+   check_morphism (nm_m1++ " refinement morphism (Partial)") (Just PartialM) f m1 af True
+   check_morphism (nm_m1++ " refinement morphism (Total)") (Just TotalM) f m1 af True
+ 
+
+-- Checks the well-formedness of refinement
+do_test3 = do
+    amdl<-load_mdl_def def_path "PersonVehicleAny"
+    mdl<-load_mdl_def def_path "PersonVehicleMotor"
+    rms<-load_rm_cmdl_def def_path "PersonVehicleMotor"
+    check_report_wf "PersonVehicleAny" (Just Total) amdl True
+    check_report_wf "PersonVehicleMotor" (Just Total) mdl True
+    check_morphism "Refinement of 'PersonVehicleMotor' by 'PersonVehicleAny'" (Just TotalM) mdl rms amdl True
+
+do_main = do
+   do_test1
+   check_PVA
+   check_PVM
+   do_test2
+   do_test3
+
+main = do
+   option_main_save do_main saveDrawings
+
+
+
+
+
