Isabelle/Fragmenta/Fragmenta_SGElemTys.thy
@@ -1,0 +1,60 @@
+(*  Theory:      SGElemTys
+    Description: Definitions related to the different types of SG elements (nodes or edges).
+    Author:     Nuno Amálio
+*)
+
+theory Fragmenta_SGElemTys
+  imports Main
+begin
+
+(* Node types of a SG: normal, abstract, proxy, enumeration, 
+  value, virtual and optional*)
+datatype SGNT = nnrml | nabst | nprxy | nenum | nval | nvirt | nopt
+datatype SGED = dbi | duni
+datatype SGET = einh | ecomp SGED | erel SGED | ewander | eder
+
+definition SGNT_set :: "SGNT set"
+where 
+   "SGNT_set = {nnrml, nabst, nprxy, nenum,  nval, nvirt, nopt}"
+
+definition erels::"SGET set"
+  where 
+  "erels = erel ` {dbi, duni}"
+
+definition ecomps::"SGET set"
+  where 
+  "ecomps = ecomp ` {dbi, duni}"
+
+definition SGET_set :: "SGET set"
+where 
+   "SGET_set = {einh, erel dbi, erel duni, 
+  ewander, eder} \<union> ecomps \<union> erels"
+
+(*Dictates allowed inheritance relations between node types*)
+definition ilt_NT::"SGNT \<Rightarrow> SGNT  \<Rightarrow> bool" (infixl "<\<^sub>N\<^sub>T" 100)
+  where
+  "nt\<^sub>1 <\<^sub>N\<^sub>T nt\<^sub>2 \<equiv> nt\<^sub>2 = nenum \<longleftrightarrow> nt\<^sub>1 = nval
+    \<and> nt\<^sub>1 = nvirt \<longrightarrow> nt\<^sub>2 = nvirt
+    \<and> nt\<^sub>1 = nabst \<longrightarrow>  nt\<^sub>2 \<in> {nabst, nprxy, nvirt}
+    \<and> nt\<^sub>1 \<notin> {nprxy, nenum} \<and> nt\<^sub>2 \<noteq> nopt"
+
+(*Dictates allowed refinement relations between node types*)
+definition rleq_NT::"SGNT \<Rightarrow> SGNT  \<Rightarrow> bool" (infixl "\<le>\<^sub>N\<^sub>T" 100)
+  where
+  "nt\<^sub>1\<le>\<^sub>N\<^sub>T nt\<^sub>2 \<equiv> nt\<^sub>1 = nt\<^sub>2 \<or> nt\<^sub>1 = nprxy 
+      \<or> nt\<^sub>2 = nabst \<and> nt\<^sub>1 \<in> {nnrml, nvirt} 
+      \<or> nt\<^sub>2 \<in> {nnrml, nopt}"
+
+
+definition eq_ET:: "SGET \<Rightarrow> SGET \<Rightarrow> bool" (infixl "=\<^sub>E\<^sub>T" 100)
+where
+  "et\<^sub>1 =\<^sub>E\<^sub>T et\<^sub>2 \<equiv> et\<^sub>1 = et\<^sub>2 \<or> ({et\<^sub>1, et\<^sub>2} \<subseteq> erels)
+    \<or> ({et\<^sub>1, et\<^sub>2} \<subseteq> ecomps)"
+
+(*Dictates allowed refinement relations between edge types*)
+definition leq_ET:: "SGET \<Rightarrow> SGET \<Rightarrow> bool" (infixl "\<le>\<^sub>E\<^sub>T" 100)
+  where
+  "et\<^sub>1 \<le>\<^sub>E\<^sub>T et\<^sub>2 \<equiv> einh \<notin>  {et\<^sub>1, et\<^sub>2}  
+    \<and> (et\<^sub>1 =\<^sub>E\<^sub>T et\<^sub>2 \<or> et\<^sub>2 = ewander 
+      \<or> (et\<^sub>1 = eder \<and> et\<^sub>2 \<in> erels \<union> ecomps))"
+end
