Haskell/FragmentaTests/GTests/G_chain_4.g
@@ -1,0 +1,9 @@
+Graph Chain_4 {
+   node V1
+   node V2
+   node V3
+   node V4
+   edge V1->V2
+   edge V2->V3
+   edge V3->V4
+}
